\documentclass{article}
\usepackage{epsfig}
\usepackage{Honeycomb}
\pagestyle{empty}
\begin{document}
$ ax + by = u $
\pagebreak

$ cx + dy = v $
\pagebreak

$ O(m n\ rhs_n) $
\pagebreak

$ M^T $
\pagebreak

$ M^T * rhs $
\pagebreak

$ M * rhs^T $
\pagebreak

$ M^T * rhs^T = (rhs*M)^T $
\pagebreak

$ v' = M_1*(M_0*v) = M_1*M_0*v $
\pagebreak

$ T(x,y,z) = [3,7,11] $
\pagebreak

$ tm = T R S $
\pagebreak

$ S = U K U^{-1} $
\pagebreak

$ v' = q_1*q_0*v $
\pagebreak

$U^{-1}$
\pagebreak

$ Rx = B$
\pagebreak

$ Ax = B $
\pagebreak

$ x = A^{-1} B = (V^T)^T W^{-1} U^T B $
\pagebreak

$ Ax = I $
\pagebreak

$ x = A^{-1} = (V^T)^T W^{-1} U^T $
\pagebreak

$ Lx = B $
\pagebreak

$(A = A^T)$
\pagebreak

$\vec{v}$
\pagebreak

$ A \vec{v} = w \vec{v} $
\pagebreak

$ A = V W V^T $
\pagebreak

$ O(n^3) $
\pagebreak

$ V^T $
\pagebreak

$ X \vec{b} = \vec{y} $
\pagebreak

$\vec{y}$
\pagebreak

$\vec{b}$
\pagebreak

$ \vec{r} = X \vec{b} - \vec{y} $
\pagebreak

$\ell^2$
\pagebreak

$ \| \vec{r} \| $
\pagebreak

$\displaystyle \min_{\vec{b}} \left\| X \vec{b} - \vec{y} \right\|_2 $
\pagebreak

$ 1 + x + x^2 = y $
\pagebreak

$(x,y)$
\pagebreak

$ b_0 + b_1 x + b_2 x^2 = y $
\pagebreak

$(1,x,x^2)$
\pagebreak

$ C \vec{b} = \vec{d} $
\pagebreak

$ c_2 x^2 + c_1 x + c_0 $
\pagebreak

$ c_1 x + c_0 = 0 $
\pagebreak

$ c_2 x^2 + c_1 x + c_0 = 0 $
\pagebreak

$ c_3 x^3 + c_2 x^2 + c_1 x + c_0 = 0 $
\pagebreak

$ c_4 x^4 + c_3 x^3 + c_2 x^2 + c_1 x + c_0 = 0 $
\pagebreak

$ A = Q R $
\pagebreak

$ A = Q \begin{bmatrix} R \\ 0 \end{bmatrix} $
\pagebreak

$ O(n^2 m) $
\pagebreak

$ A = U W V^T $
\pagebreak

$\mathrm{Beta}$
\pagebreak

$ p(x) = \mathrm{Beta}(x+1, n-x+1) $
\pagebreak

$\displaystyle p(x,\alpha,\beta) = \frac{x^{\alpha-1} (1-x)^{\beta-1}}{\mathrm{B}(\alpha,\beta)} $
\pagebreak

$\alpha$
\pagebreak

$\beta$
\pagebreak

$\displaystyle p(x,n,p) = \binom{n}{x} p^x (1-p)^{n-x} $
\pagebreak

$\displaystyle \binom{n}{k} = \frac{n!}{k!(n-k)!} $
\pagebreak

$\displaystyle p(x,n,p) = \frac{\Gamma(n+x)}{\Gamma(n) \Gamma(x+1)} p^n (1-p)^x $
\pagebreak

$\Gamma$
\pagebreak

$\chi^2$
\pagebreak

$\displaystyle \chi^2 = \sum_{i=1}^6 \frac{observedFreq_i - expectedFreq_i^2}{expectedFreq_i} $
\pagebreak

$ p = 1 - cdf(\chi^2, 6-1) $
\pagebreak

$\lambda = 0$
\pagebreak

$\mathrm{Gamma}(\nu/2, 2)$
\pagebreak

$\displaystyle p(x,\nu,\lambda) = \frac{1}{2^{\nu/2} \Gamma(\nu/2)} x^{\nu/2 - 1} e^{-x/2} $
\pagebreak

$\lambda \not= 0$
\pagebreak

$\displaystyle p(x,\nu,\lambda) = \sum_{i=0}^\infty \frac{e^{-\lambda/2} (\lambda/2)^i}{i!} \chi^2(x, \nu+2i) $
\pagebreak

$\nu$
\pagebreak

$\lambda$
\pagebreak

$\mathrm{Gamma}$
\pagebreak

$\displaystyle p(x,\alpha,\beta) = \frac{1}{\Gamma(\alpha) \beta^\alpha} x^{\alpha-1} e^{-x / \beta} $
\pagebreak

$\theta$
\pagebreak

$\displaystyle p(x,\mu,\sigma) = \frac{1}{\sigma \sqrt{2\pi}} e^{-\frac{(x-\mu)^2}{2\sigma^2}} $
\pagebreak

$\mu$
\pagebreak

$\sigma$
\pagebreak

$\displaystyle p(x,n,m,N) = \frac{C(m,x) C(N-m, n-x)}{C(N,m)} $
\pagebreak

$\displaystyle p(x,\mu) = \frac{\mu^x e^{-\mu}}{x!} $
\pagebreak

$\displaystyle p(x,n) = \frac{\Gamma \paren*{ \frac{n+1}{2}} } {\sqrt{n\pi} \; \Gamma \paren*{ \frac{n}{2} }} \paren*{1 + \frac{x^2}{n}}^{\!\! -\frac{n+1}{2}} $
\pagebreak

$\displaystyle p(x,\alpha,\beta) = \frac{\beta}{\alpha} \paren*{ \frac{x}{\alpha} }^{\beta-1} e^{-(x/\alpha)^\beta} $
\pagebreak

\end{document}
